---
title: "ADI symbolic"
format:
  html:
    code-fold: true
jupyter: python3
---


```{python}
from sympy import *
```


```{python}
Nx = 4
Ny = 5

uk = MatrixSymbol("u^{k}", Nx+1, Ny+1)
ukp1 = MatrixSymbol("u^{k+1}", Nx+1, Ny+1)
```

```{python}
rx = symbols("r_x")
ry = symbols("r_y")
```

## Kasus $j=1$

```{python}
eqn_list = []
j = 1
for i in range(1,Nx):
    lhs = -ry*(ukp1[i,j+1] + ukp1[i,j-1]) + (1 + 2*ry)*ukp1[i,j]
    rhs = rx*(uk[i+1,j] + uk[i-1,j]) + (1 - 2*rx)*uk[i,j]
    eqn = Equality(lhs, rhs)
    eqn_list.append(eqn)
```

```{python}
for eqn in eqn_list:
    print(latex(eqn))
```

Manually copy the result here:
$$
- r_{y} \left(u^{k+1}_{1, 0} + u^{k+1}_{1, 2}\right) + \left(2 r_{y} + 1\right) u^{k+1}_{1, 1} = r_{x} \left(u^{k}_{0, 1} + u^{k}_{2, 1}\right) + \left(1 - 2 r_{x}\right) u^{k}_{1, 1}
$$

$$
- r_{y} \left(u^{k+1}_{2, 0} + u^{k+1}_{2, 2}\right) + \left(2 r_{y} + 1\right) u^{k+1}_{2, 1} = r_{x} \left(u^{k}_{1, 1} + u^{k}_{3, 1}\right) + \left(1 - 2 r_{x}\right) u^{k}_{2, 1}
$$

$$
- r_{y} \left(u^{k+1}_{3, 0} + u^{k+1}_{3, 2}\right) + \left(2 r_{y} + 1\right) u^{k+1}_{3, 1} = r_{x} \left(u^{k}_{2, 1} + u^{k}_{4, 1}\right) + \left(1 - 2 r_{x}\right) u^{k}_{3, 1}
$$


```{python}
eqn_list[1]
```

Search for boundary points:
```{python}
bc_pts_list = []
ip = 0
for i in range(Nx+1):
    for j in range(Ny+1):
        if (i == 0) or (i == Nx):
            bc_pts_list.append(ip)
        elif (j == 0) or (j == Ny):
            bc_pts_list.append(ip)
        ip += 1
```

Index-$i = 0$ dan indeks-$i=N_x$ adalah BC.

Index-$j = 0$ dan indeks-$j=N_y$ adalah BC.

## Kasus $j=2$

```{python}
eqn_list = []
j = 2
for i in range(1,Nx):
    lhs = -ry*(ukp1[i,j+1] + ukp1[i,j-1]) + (1 + 2*ry)*ukp1[i,j]
    rhs = rx*(uk[i+1,j] + uk[i-1,j]) + (1 - 2*rx)*uk[i,j]
    eqn = Equality(lhs, rhs)
    eqn_list.append(eqn)
```

```{python}
for eqn in eqn_list:
    print(latex(eqn))
```

$$
- r_{y} \left(u^{k+1}_{1, 1} + u^{k+1}_{1, 3}\right) + \left(2 r_{y} + 1\right) u^{k+1}_{1, 2} = r_{x} \left(u^{k}_{0, 2} + u^{k}_{2, 2}\right) + \left(1 - 2 r_{x}\right) u^{k}_{1, 2}
$$

$$
- r_{y} \left(u^{k+1}_{2, 1} + u^{k+1}_{2, 3}\right) + \left(2 r_{y} + 1\right) u^{k+1}_{2, 2} = r_{x} \left(u^{k}_{1, 2} + u^{k}_{3, 2}\right) + \left(1 - 2 r_{x}\right) u^{k}_{2, 2}
$$

$$
- r_{y} \left(u^{k+1}_{3, 1} + u^{k+1}_{3, 3}\right) + \left(2 r_{y} + 1\right) u^{k+1}_{3, 2} = r_{x}
\left(u^{k}_{2, 2} + u^{k}_{4, 2}\right) + \left(1 - 2 r_{x}\right) u^{k}_{3, 2}
$$